Added associativity proof for tp

meta_subst.v
@@ -2,11 +2,20 @@ Require Import util.
 Require Import worlds. 
 Require Import meta_term.
 
-Definition msubst δ δ' := name δ -> meta_term δ'.
-Class substitutable (A:world -> Set) := 
-   app_subst : forall {α β}, msubst α β -> A α -> A β.
+Class substitutable (A:world -> Set) := {
+   app_subst : forall {α β}, msubst α β -> A α -> A β ;
+   assoc : forall {α} (t:A α) {β} (θ:msubst α β) {γ} (θ':msubst β γ), app_subst θ' (app_subst θ t) = app_subst (app_msubst θ' ○ θ) t
+ }.
 Notation "⟦ θ ⟧" := (app_subst θ). 
-Typeclasses Transparent substitutable.
-Typeclasses Transparent app_subst.
 
+Instance meta_term_substitutable : substitutable meta_term := { app_subst := app_msubst;
+   assoc := @app_msubst_assoc
+ }.
+Instance mtype_substitutable : substitutable mtype := {
+  app_subst := app_msubst_mtype;
+  assoc := @app_msubst_mtype_assoc
+ }.
+
+Definition import_meta_term {δ δ'} (y:δ↪δ') : meta_term δ -> meta_term δ' := ⟦import y⟧.
+Definition import_mtype {δ δ'} (y:δ↪δ') : mtype δ -> mtype δ' := ⟦import y⟧.
 Hint Transparent app_subst.
