meta_subst_type.v
@@ -1,4 +1,5 @@
 Require Import util.
+Require Import Coq.Logic.FunctionalExtensionality.
 Require Import worlds.
 Require Import meta_subst.
 Require Import comp_expr.
@@ -6,16 +7,18 @@ Require Import meta_subst_meta_type.
 Require Import meta_subst_meta_term.
 Require Import meta_subst_typing.
 Require Import meta_term.
-
+Require Import meta_subst_meta_subst.
+Require Import Setoid.
 
 Definition import_msubst {δ δ' δ''} (X:δ'↪δ'')  (θ:msubst δ δ')  : msubst δ δ'' :=
  import_meta_term X ○ θ.
 
-Section app_msubst_t2_sect.
+Section app_msubst_tp_sect.
 
 Reserved Notation "[ θ ] T" (at level 90).
-
-Fixpoint app_msubst_t2 {ψ} {δ δ'} (θ:msubst δ δ') (T:tp' ψ δ) : tp' ψ δ' :=
+Definition context_mult {δ δ'} (θ:msubst δ δ') {δ'' δ'''} (y:δ'↪δ''') (x:δ↪δ'') := (import_msubst y θ,, (x,m_var y)).
+Notation "θ × ( y // x )" := (context_mult θ y x) (at level 10).
+Fixpoint app_msubst_tp {ψ} {δ δ'} (θ:msubst δ δ') (T:tp' ψ δ) : tp' ψ δ' :=
 match T  with
  | m_tp U     =>
    m_tp _ (⟦θ⟧ U)
@@ -23,10 +26,10 @@ match T  with
    arr ([θ] T1) ([θ] T2)
  | pi _ X U T0 =>
    let (_,X') := next δ' in
-   pi X' (⟦θ⟧ U) ([import_msubst X' θ,, (X,m_var X')] T0)
+   pi X' (⟦θ⟧ U) ([ θ × (X' // X )] T0)
  | sigma _ X U T0 =>
    let (_,X') := next δ' in
-   sigma X' (⟦θ⟧ U) ([import_msubst X' θ,, (X,m_var X')] T0)
+   sigma X' (⟦θ⟧ U) ([ θ × (X' // X )] T0)
  | unit =>
    unit _ _
  | prod T1 T2 =>
@@ -40,12 +43,70 @@ match T  with
  | eq_constraint C1 C2 T0 =>
    eq_constraint (⟦θ⟧ C1) (⟦θ⟧ C2) ([θ] T0)
 end
-where "[ θ ] T" := (app_msubst_t2 θ T).
-End app_msubst_t2_sect.
-Implicit Arguments app_msubst_t2.
+where "[ θ ] T" := (app_msubst_tp θ T).
 
+Instance tp_substitutable' : substitutable tp := {
+  app_subst := @app_msubst_tp empty
+}.
+pose proof (@assoc _ mtype_substitutable).
+pose proof (@assoc _ meta_term_substitutable).
+unfold app_subst in *. unfold mtype_substitutable in *.
+unfold meta_term_substitutable in *.
 
- Instance tp_substitutable : substitutable tp := (@app_msubst_t2 empty).
+intros α T. induction T; intros;
+simpl;
+f_equal; firstorder.
+remember (next' γ).
+remember (next' β).
+destruct s0.
+destruct s1.
+simpl.
+erewrite IHT.
+f_equal.
+eapply functional_extensionality_dep.
+intro. unfold compose at 1.
+unfold context_mult at 2.
+unfold compose at 1.
 
-Axiom msubst_single_t : forall {D D'} (X:wlink D D'), meta_term D -> tp D' -> tp D.
-(* TODO: Write this as a simultaneous substitution: (id,C/X) ? *)
+unfold context_mult at 2.
+unfold compose at 1.
+
+remember (export s x1).
+destruct s2; simpl in *.
+unfold import_msubst.
+unfold import_meta_term.
+unfold app_subst.
+unfold meta_term_substitutable.
+unfold compose at 1.
+erewrite H0.
+unfold compose at 1.
+assert ((fun a => app_msubst (θ' ×  (s0 // s1)) (m_var (import s1 a))) = import_msubst s0 θ').
+eapply functional_extensionality_dep.
+intro.  erewrite app_msubst_mvar_result.
+unfold context_mult.
+unfold compose.
+erewrite export_import_inv.
+simpl.
+reflexivity.
+rewrite H1.
+unfold compose.
+erewrite H0.
+unfold import_msubst.
+unfold import_meta_term.
+unfold app_subst.
+unfold meta_term_substitutable.
+reflexivity.
+
+unfold context_mult.
+unfold compose.
+erewrite app_msubst_mvar_result.
+erewrite export_self. reflexivity.
+admit. (* TODO: Extract lemma. (It's the same proof) *)
+Defined.
+End app_msubst_tp_sect.
+Implicit Arguments app_msubst_tp.
+
+Instance tp_substitutable : substitutable tp := tp_substitutable'.
+
+Definition msubst_single_t {δ δ'} (X:δ↪δ') (t:meta_term δ) : tp δ' -> tp δ :=
+ ⟦ (maybe (@m_var _ ) t) ○ (export X) ⟧.
