meta_term.v
@@ -6,10 +6,6 @@ Require Import util.
  Coercion m_var : name >-> meta_term.
  Implicit Arguments m_var [δ].
 
- Axiom import_meta_term : forall {δ δ'}, δ↪δ' -> meta_term δ -> meta_term δ'.
-
- Axiom import_mtype : forall {δ δ'}, δ↪δ' -> mtype δ -> mtype δ'.
-
  Open Scope type_scope.
  Definition mtype_assign δ := name δ -> mtype δ.
 
@@ -17,4 +13,25 @@ Require Import util.
  Implicit Arguments m_oft.
 
  Notation "D ⊨ t ∷ U" := (m_oft D t U) (at level 90).
+
+Definition msubst δ δ' := name δ -> meta_term δ'.
+
+Axiom app_msubst : forall {δ δ'}, (msubst δ δ') -> meta_term δ -> meta_term δ'.
+
+Axiom app_msubst_assoc : forall {δ} (t:meta_term δ)
+ {δ'} (θ:msubst δ δ') {δ''} (θ':msubst δ' δ''),
+ app_msubst θ' (app_msubst θ t) =
+ app_msubst (app_msubst θ' ○ θ) t.
+Implicit Arguments app_msubst.
+Axiom app_msubst_mtype : forall {δ δ'}, (msubst δ δ') -> mtype δ -> mtype δ'.
+Axiom app_msubst_mtype_assoc : forall {δ} (U:mtype δ)
+ {δ'} (θ:msubst δ δ') {δ''} (θ':msubst δ' δ''),
+  app_msubst_mtype θ' (app_msubst_mtype θ U) =
+  app_msubst_mtype (app_msubst θ' ○ θ) U.  
+
+Implicit Arguments app_msubst_mtype.
+
+
+Axiom app_msubst_mvar_result : forall {δ δ'} (θ:msubst δ δ')
+  (n:name δ), app_msubst θ  (m_var n) = θ n.
 
