meta_subst_meta_subst.v
@@ -1,8 +1,20 @@
 Require Import util.
+Require Import Coq.Logic.FunctionalExtensionality.
 Require Import worlds.
+Require Import meta_term.
 Require Import meta_subst.
 Require Import meta_subst_meta_term.
  
 Instance msubst_substitutable {δ} : substitutable (msubst δ)
-  := fun _ _ θ θ' => ⟦θ⟧ ○ θ'.
- 
+  := {
+  app_subst := fun _ _ θ θ' => ⟦θ⟧ ○ θ'
+  }.
+intros. 
+pose proof (@assoc _ meta_term_substitutable).
+unfold app_subst in *.
+unfold meta_term_substitutable in *.
+extensionality x.
+unfold compose in *.
+erewrite H.
+reflexivity.
+Defined.
