meta_subst_meta_term.v
@@ -4,13 +4,3 @@ Require Import meta_subst.
 Require Import meta_term.
 Require Import meta_subst_typing.
 
-Axiom app_msubst : forall W W', msubst W W' -> meta_term W -> meta_term W'.
-
-Definition app_msubst_mvar {δ δ'} (θ:msubst δ δ') : name δ -> meta_term δ' := fun n => θ n.
-
-Implicit Arguments app_msubst.
-Instance meta_term_substitutable : substitutable meta_term :=
- app_msubst.
-
-Axiom app_msubst_mvar_result : forall {δ δ'} (θ:msubst δ δ')
-  (n:name δ), ⟦ θ ⟧ (m_var n) = app_msubst_mvar θ n.
